\documentclass{article}
\usepackage{amsmath}
\usepackage{amssymb}
\usepackage{amsthm}
\usepackage{graphicx}
\usepackage{tikz}
\usepackage{tikz-cd}
\usepackage{enumerate}
\usepackage{color}
\usepackage{hyperref}
\usepackage{enumerate}

\author{Adrian Lozada, U71130053}
\title{Quiz 3}
\date{October 10, 2019}

\begin{document}
    \maketitle
    \newpage
    \section{Problem 1}
    \begin{flushleft}
        1. Find the general solution to the differential equation
    \end{flushleft}
    \begin{equation}
        y'' + 6y' + 9y = x^{2} + \cos(x) - xe^{-3x}
    \end{equation}
        $Homogeneous$ $Equation:$
    \begin{align*}
        y'' + 6y' + 9y &= 0 \\
    \end{align*}
        $Characteristic$ $Equation:$
    \begin{align*}
        r^{2} + 6r + 9 &= 0 \\
        (r + 3)(r + 3) &= 0 \\
        r &= -3
    \end{align*}
        $Homogeneous$ $Solution:$
    \begin{align*}
        y_{h} &= \frac{(A + Bx)}{e^{3x}}\\
    \end{align*}

        $Particular$ $Solution$ $1:$
    \begin{align*}
        y'' + 6y' + 9y &= \cos{x} \\
    \end{align*}
        $$m = 0, \alpha = 0, k = 0, s = 0, \beta = 1, C = 1$$
    \begin{align*}
        y_{p1} = A\cos{x} + B\sin{x} \\
    \end{align*}
        Solving for the constants:
    \begin{align*}
        \begin{cases}
            [9] \quad y_{p1} = A\cos{x} + B\sin{x} \\
            [6] \quad y_{p1}' = -A\sin{x} + B\cos{x} \\
            [1] \quad y_{p1}'' = -A\cos{x} - B\sin{x} \\
        \end{cases}
    \end{align*}

    \begin{align*}
        \cos{x}: \quad &9A + 6B - A = 1 \\
        & 8A + 6B = 1\\
        & A = \frac{1 - 6B}{8} \\
        \sin{x}: \quad &9B -A6 - B = 0 \\
        & 8B - 6A = 0 \\
        & 8B - 6\left(\frac{1 - 6B}{8}\right) = 0 \\
        & 100B = 6 \\
        & B = \frac{6}{100} = \frac{3}{50}\\
        & A = \frac{2}{25} \\
    \end{align*}
    \begin{align*}
        y_{p1} = \frac{2}{25}\cos{x} + \frac{3}{50}\sin{x} \\
    \end{align*}
    $Particular$ $Solution$ $2:$
    \begin{align*}
        y'' + 6y' + 9y &= x^{2} \\
    \end{align*}
        $$m = 2, \alpha = 0, s = 0, C = 1$$
    \begin{align*}
        y_{p2} = Ax^{2} + Bx + C\\
    \end{align*}

        Solving for the constants:
    \begin{align*}
        \begin{cases}
           [9] \quad y_{p2} = Ax^{2} + Bx + C \\
            [6] \quad y_{p2}' = 2Ax + B \\
            [1] \quad y_{p2}'' = 2A \\
        \end{cases}
    \end{align*}
    \begin{align*}
        x^{2}: \quad & 9A = 1 \\
        & A = \frac{1}{9} \\
        x: \quad & 9B + 12A = 0 \\
        & 9B = -12A \\
        & 9B = -\frac{12}{9} \\
        & 9B = -\frac{4}{3} \\
        & B = -\frac{4}{27} \\
        1: \quad & 9C + 6B + 2A = 0 \\
        & 9C + 6\left(-\frac{4}{27}\right) + 9\left(\frac{1}{9}\right) = 0 \\
        & 9C - \frac{8}{9} + \frac{2}{9} = 0 \\
        & 9C - \frac{8}{9} = -\frac{2}{9} \\
        & 9C = \frac{6}{9} \\
        & C = \frac{2}{27} \\
    \end{align*}
    \begin{align*}
        y_{p2} = \frac{1}{9}x^{2} - \frac{4}{27}x + \frac{2}{27} \\
    \end{align*}
    $Particular$ $Solution$ $3:$
    \begin{align*}
        y'' + 6y' + 9y &= xe^{-3x} \\
    \end{align*}
        $$m = 0, \alpha = 0, k = 0, s = 0, \beta = 1, C = 1$$
    \begin{align*}
        y_{p3} = \frac{(Ax^{3} + Bx^{2})}{e^{3x}}\\
    \end{align*}
        Solving for the constants:
    \begin{align*}
        \begin{cases}
            [9] \quad y_{p3} = \frac{(Ax^{3} + Bx^{2})}{e^{3x}} \\
            [6] \quad y_{p3}' = \frac{(3Ax^{2} + 2Bx - 3Ax^3 -3Bx^{2})}{e^{3x}} \\
            [1] \quad y_{p3}'' = \frac{(6Ax + 2B - 9Ax^{2} -6Bx -9Ax^{2} -6Bx + 9Ax^{3} + 9Bx^{2})}{e^{3x}} \\
        \end{cases}
    \end{align*}
    \begin{align*}
        &x^{3}: 9A -18A + 9A = 0\\
        &x^{2}: 9B - 18B + 9B -9A + 18A - 9A = 0\\
        &x: 12B + 6A - 12B = -1\\
        &6A = -1\\
        &A = -\frac{1}{6}\\
        &B = 0 \\
    \end{align*}
    \begin{align*}
        y_{p3} = \frac{(-\frac{1}{6})x^{3}}{e^{3x}}\\
    \end{align*}
    \begin{align*}
        y = y_{h} + y_{p1} + y_{p2} + y_{p3} \\
    \end{align*}


    \newpage
    \section{Problem 2}
    \begin{flushleft}
        2. Find the general solution to the differential equation
    \end{flushleft}
    \begin{equation}
        y'' - 2y' + 5y = xe^{x} + xe^{x}\sin{(2x)}
    \end{equation}
    $Homogeneous$ $Equation:$
    \begin{align*}
        y'' - 2y' + 5y &= 0 \\
    \end{align*}
    \begin{align*}
        &r = x^{2} - 2x + 5 \\
        &r = \frac{2 \pm i4}{2} \\
        &\alpha = 1, \beta = 2
    \end{align*}
        $Homogeneous$ $Solution:$
    \begin{align*}
        y_{h} &= e^{x}(A\cos{(2x)} + B\sin{(2x)}) 
    \end{align*}    
    $Particular$ $Solution$ $1:$
    \begin{align*}
        y'' - 2y' + 5y &= xe^{x}\\
    \end{align*}
        $$m = 1, \alpha = 1, s = 0, C = 1$$
    \begin{align*}
        y_{p1} &= (Ax + B)e^{x} \\
    \end{align*}
        Solving for the constants:
    \begin{align*}
        \begin{cases}
            [5] \quad y_{p1} = (Ax + B)e^{x} \\
            [-2] \quad y_{p1}' = (Ax + B + A)e^{x} \\
            [1] \quad y_{p1}'' = (Ax + B + 2A)e^{x} \\
        \end{cases}
    \end{align*}
    \begin{align*}
        x: \quad & 5A -2A + A = 1 \\
        & A = \frac{1}{4} \\
        &B = 0
    \end{align*}
    \begin{align*}
        y_{p1} = \frac{1}{4}xe^{x} \\
    \end{align*}


    $Particular$ $Solution$ $2:$
    \begin{align*}
        y'' - 2y' + 5y &= xe^{x}\sin{2x}\\
    \end{align*}
        $$m = 1, \alpha = 1, s = 0, C = 1, \beta = 2$$
    \begin{align*}
        y_{p1} &= xe^{x}((Ax + B)\cos{2x} + (Cx + D)\sin{(2x)}) \\
    \end{align*}
        Solving for the constants:
    \begin{align*}
        \begin{cases}
            [5] \quad y_{p2} = xe^{x}((Ax + B)\cos{2x} + (Cx + D)\sin{(2x)}) \\
            [-2] \quad y_{p2}' = e^{x}((C - 2A)x^2 + (D + 2C  -3B)x  + D)\sin{2x} + e^{x}((2C + A)x^2 + (2D + B + 2A)x + B)\cos{2x} \\
            [1] \quad y_{p2}'' = ((-3C -4A)x^2 + (-3D + 4C - 4B -8A)x + 2D + 2C -4B)e^{x}\sin{2x} + \\ ((4C-3A)x^2 + (4D + 8C -3B  + 4A)x  + 4D + 2B + 2A)e^{x}\cos{2x} \\
        \end{cases}
    \end{align*}

    \begin{align*}
        x^2: & 5A + 5C - 2C +4A -4A -2C + -2A -3C -4A +4C -3A = 0 \\
        x: & 5B + 5D + -2D -4C +6B -4D -2B -4A  -3D +4C -4B -8A +4D +8C -3B +4A= 1 \\
        & A = -\frac{1}{8} \\
        &B = 0 \\
        &C = 0 \\
        &D = \frac{1}{16} \\
    \end{align*}
    \begin{align*}
        y_{p2} = xe^{x}\left( \frac{\sin{(2x)}}{16} - \frac{x\cos{(2x)}}{8}\right)\\
    \end{align*}
    \begin{align*}
        y = y_{h} + y_{p1} + y_{p2} \\
    \end{align*}





\end{document}