\documentclass{article}
\usepackage{amsmath}
\usepackage{amssymb}
\usepackage{amsfonts}
\usepackage{graphicx}
\usepackage{hyperref}
\usepackage{enumerate}
\usepackage{float}
\usepackage{caption}
\usepackage{subcaption}
\usepackage{tikz}
\usepackage{pgfplots}
\usepackage{pgfplotstable}
\usepackage{fancyhdr}
\usepackage{mathtools}
\usepackage{setspace}


\renewcommand{\maketitle}{
    \begin{center}
        \begin{tabular}{c}
            \textbf{Quiz 2} \\
            \textbf{Adrian Lozada} \\
            \textbf{U71130053} \\
        \end{tabular}
    \end{center}
}

% Enumerate the pages in the document
\pagenumbering{arabic}
\allowdisplaybreaks

\begin{document}
    \maketitle
    
    % First problem
    \newpage
    \begin{flushleft}
        \textbf{Q.1 Solve the following differential equation:}
    \end{flushleft}
    \begin{center}
        \begin{equation}
            \left( 3e^{3x}\ln{(1+y^{2})}-\frac{x}{\sqrt[2]{x^{2}+1}} \right)dx 
            =
            \left(2\sin{(y)}cos{(y)}-2e^{3x}\frac{y}{1+y^{2}}\right)dy
        \end{equation}
    \end{center}
    \begin{flushleft}
        where $y(0)=0$
    \end{flushleft}
    \begin{flushleft}
        Exactness Condition:
    \end{flushleft}
    \begin{equation}
        \frac{\partial M}{\partial y} = \frac{\partial N}{\partial x}
    \end{equation}
    \begin{equation}
        M = 3e^{3x}\ln{(1+y^{2})}-\frac{x}{\sqrt[2]{x^{2}+1}}
    \end{equation}
    \begin{equation}
        N = -2\sin{(y)}cos{(y)}+2e^{3x}\frac{y}{1+y^{2}}
    \end{equation}
    \begin{equation}
        \frac{\partial M}{\partial y} = \frac{6ye^{3x}}{1+y^{2}}
        \qquad
        \frac{\partial N}{\partial x} = \frac{6ye^{3x}}{1+y^{2}}
    \end{equation}
    % Solving the differential equation
    \begin{flushleft}
        Therefore, the differential equation is exact.
    \end{flushleft}
    \begin{flushleft}
        Solution:
    \end{flushleft}
    \begin{equation}
        \left( 3e^{3x}\ln{(1+y^{2})}-\frac{x}{\sqrt[2]{x^{2}+1}} \right)dx 
        -
        \left(2\sin{(y)}cos{(y)}-2e^{3x}\frac{y}{1+y^{2}}\right)dy = 0
    \end{equation}
    \begin{equation}
        \left( 3e^{3x}\ln{(1+y^{2})}-\frac{x}{\sqrt[2]{x^{2}+1}} \right)dx 
        +
        \left(-2\sin{(y)}cos{(y)}+2e^{3x}\frac{y}{1+y^{2}}\right)dy = 0
    \end{equation}
    \begin{equation}
        \frac{\partial F}{\partial x} = M 
        \qquad
        \frac{\partial F}{\partial y} = N
    \end{equation} 
    \begin{equation}
            \int \frac{\partial F}{\partial x}dx 
            = 
            \int \left( 3e^{3x}\ln{(1+y^{2})}-\frac{x}{\sqrt[2]{x^{2}+1}} \right)dx
    \end{equation}
    \newpage
    \begin{singlespace}
        \begin{align*}
            &= \int \left(3e^{3x}\ln(1+y^{2})\right)dx  - \int \left(\frac{x}{\sqrt[2]{x^{2}+1}}\right)dx \\
            &= e^{3x}\ln(1+y^{2}) - \int \left(\frac{x}{\sqrt[2]{x^{2}+1}}\right)dx \\
        \end{align*}
        $u=x^{2}+1$ so that $du=2xdx$ and $dx=\frac{du}{2x}$
        \begin{align*}
            &= e^{3x}\ln(1+y^{2}) - \int \left(\frac{1}{2\sqrt[2]{u}}\right)du \\
            &= e^{3x}\ln(1+y^{2}) - \sqrt[2]{u} + f(y) \\
            &= e^{3x}\ln(1+y^{2}) - \sqrt[2]{x^{2}+1} + f(y) \\
        \end{align*}
        \begin{flushleft}
            Hence, F equals:
        \end{flushleft}
        \begin{equation}
            F(x, y) = e^{3x}\ln(1+y^{2}) - \sqrt[2]{x^{2}+1} + f(y)
        \end{equation}
        \begin{flushleft}
            Now, we solve for $f(y)$:
        \end{flushleft}
        \begin{align*}
            &\frac{\partial{F}}{\partial{y}} 
            = \frac{\partial{}}{\partial{y}}\left( e^{3x}\ln(1+y^{2}) - \sqrt[2]{x^{2}+1} + f(y) \right) \\
            &= \frac{2ye^{3x}}{1+y^{2}} + f'(y) \\
        \end{align*}
        \begin{flushleft}
            Therefore, $f'(y)$ equals:
        \end{flushleft}
        \begin{align*}
            &\frac{2ye^{3x}}{1+y^{2}} + f'(y) = \left( -2\sin(y)\cos(y) + \frac{2ye^{3x}}{1+y^{2}}\right) \\
            &f'(y) = -2\sin(y)\cos(y) \\
        \end{align*}
        \begin{flushleft}
            We integrate $f'(y)$:
        \end{flushleft}
        \begin{align*}
            &\int f'(y)dy = \int -2\sin(y)\cos(y)dy \\
            &= -\int \sin(2y)dy \\
            &= \frac{\cos(2y)}{2} \\ 
        \end{align*}
        \begin{flushleft}
            Therefore, $f(y)$ equals:
        \end{flushleft}
        \begin{align*}
            &f(y) = \frac{\cos(2y)}{2} \\
        \end{align*}
        \begin{flushleft}
            Finally, $F(x, y)$ equals:
        \end{flushleft}
        \begin{align*}
            &F(x, y) = e^{3x}\ln(1+y^{2}) - \sqrt[2]{x^{2}+1} + \frac{\cos(2y)}{2} = C_1 \\
        \end{align*}
    \end{singlespace}

    % Second problem:
    \newpage
    \begin{singlespace}
        \begin{flushleft}
            \textbf{Q.2 Find the general solution to}
        \end{flushleft}
        \begin{center}
            \begin{equation}
                \left( y-x \right)dx - \left( y +x \right)dy = 0
            \end{equation}
        \end{center}
        \begin{flushleft}
            Solution to homogeneous differential equation:
        \end{flushleft}
        \begin{align*}
            &\left( y +x \right)dy = \left( y-x \right)dx  \\
            &\frac{dy}{dx} = \frac{y-x}{y+x}
        \end{align*}
        \begin{flushleft}
            Setting up the equation in the form $u=\frac{y}{x}$:
        \end{flushleft}
        \begin{align*}
            &\frac{dy}{dx} = \frac{y-x}{y+x} * \frac{\frac{1}{x}}{\frac{1}{x}} \\
            &= \frac{\frac{y}{x}-1}{\frac{y}{x}+1} \\
            &= \frac{u-1}{u+1} \\
        \end{align*}
        \begin{flushleft}
            Therefore, $g(u)=\frac{u-1}{u+1}$ and now we set up $g(u)-u$:
        \end{flushleft}
        \begin{align*}
            &g(u)-u = \frac{u-1}{u+1} - u \\
            &= \frac{u-1}{u+1} - u\frac{u-1}{u+1} \\
            &= \frac{u-1}{u+1} - \frac{u^{2}-u}{u+1} \\
            &= \frac{u-1-u^{2}+u}{u+1} \\
            &= \frac{-u^{2}-1}{u+1} \\
        \end{align*}
        \begin{flushleft}
            Now, we set up $g(u)-u=x\frac{du}{dx}$ and integrate $\frac{dx}{x}=\frac{du}{g(u)-u}$:
        \end{flushleft}
        \begin{align*}
            &\frac{dx}{x} = \frac{du}{g(u)-u} \\
            &\int \frac{dx}{x} = \int \frac{du}{g(u)-u} \\
            &\ln(x) = \int \frac{du}{g(u)-u} \\
            &\ln(x) = \int \frac{du}{\frac{-u^{2}-1}{u+1}} \\
            &\ln(x) = \int -\frac{u+1}{u^{2}+1}du \\
            &\ln(x) = -\int \left( \frac{u}{u^{2}+1}+\frac{1}{u^{2}+1}\right)du
        \end{align*}
        \begin{flushleft}
            Now, we solve the integral $\int \frac{u}{u^{2}+1}du$:\\
        \end{flushleft}
        \begin{align*}
            &\int \frac{u}{u^{2}-1}du = \int \frac{u}{u^{2}+1}du \\
        \end{align*}
        \begin{center}
            We substitute $t=u^{2}+1$ and $dt=2udu$:
        \end{center}
        \begin{align*}
            & \int \frac{u}{u^{2}+1}du = \int \frac{u}{t}\frac{dt}{2u} \\
            &= \frac{1}{2}\int \frac{dt}{t} \\
            &= \frac{1}{2}\ln(t) \\
            &= \frac{1}{2}\ln|u^{2}+1| \\
        \end{align*}
        \begin{flushleft}
            Now, we solve the integral $\int \frac{1}{u^{2}+1}du$:\\
        \end{flushleft}
        \begin{align*}
            & \int \frac{1}{u^{2}+1}du=\arctan(u)
        \end{align*}
        \begin{flushleft}
            Therefore:
        \end{flushleft}
        \begin{align*}
            &\ln|x| = -\left(\frac{1}{2}\ln|u^{2}+1| + \arctan(u)\right) \\
            &\ln|x| = -\frac{1}{2}\ln|\frac{y^{2}}{x^{2}}+1|- \arctan\left(\frac{y}{x}\right) \\
        \end{align*}
    \end{singlespace}
\end{document}